

Q) Given that 'f' and 'g' are convex functions, prove that $f-g$ is not necessarily convex.

Sol:

We know that for any convex function 'h',

$$h(\lambda x + (1-\lambda)y) \leq \lambda h(x) + (1-\lambda)h(y)$$

for all $x, y \in \mathbb{R}$ and $\lambda \in [0, 1]$.

Now consider a f^n : $h(x) = f(x) - g(x)$

Let us say that this func. is a convex f^n

$\Rightarrow \exists t \in [0, 1]$ s.t.

$$h(tx + (1-t)y) \leq t h(x) + (1-t) h(y)$$

$$\begin{aligned} \Rightarrow f(tx + (1-t)y) - g(tx + (1-t)y) \\ \leq t[f(x) - g(x)] + (1-t)[f(y) - g(y)] \end{aligned}$$

but since 'f' is convex, we know that

$$f(tx + (1-t)y) \leq t f(x) + (1-t) f(y)$$

$$\Rightarrow -g(tx + (1-t)y) \leq -t g(x) - (1-t) g(y)$$

$$\Rightarrow g(tx + (1-t)y) \geq t g(x) + (1-t) g(y)$$

\hookrightarrow this contradicts the fact that 'g' is convex

$$\text{ie. } g(tx + (1-t)y) \leq t g(x) + (1-t) g(y)$$

\Rightarrow 'f-g' need not be convex if 'f' & 'g' are convex.

